AbstractPlatform/Types.bpl
@@ -150,16 +150,16 @@ axiom (forall o : tap_proof_op_t ::
         
 function tap_proof_op_valid(o : tap_proof_op_t) : bool 
 {
-    // false
-    o == tap_proof_op_compute ||    
-    o == tap_proof_op_destroy ||   
-    o == tap_proof_op_enter   ||   
-    o == tap_proof_op_exit    ||   
-    o == tap_proof_op_launch  ||  
-    o == tap_proof_op_resume  ||
-    o == tap_proof_op_pause   ||
-    o == tap_proof_op_release ||
-    o == tap_proof_op_block
+    false
+    // o == tap_proof_op_compute     
+    // o == tap_proof_op_destroy    
+    // o == tap_proof_op_enter   
+    // o == tap_proof_op_exit    
+    // o == tap_proof_op_launch  
+    // o == tap_proof_op_resume  
+    // o == tap_proof_op_pause  
+    // o == tap_proof_op_release 
+    // o == tap_proof_op_block
 }
 
 function tap_proof_op_valid_in_enclave(o : tap_proof_op_t) : bool
@@ -171,18 +171,18 @@ function tap_proof_op_valid_in_enclave(o : tap_proof_op_t) : bool
 }
 
 /* proved: exit pause launch resume destroy */
-/* todo: compute enter resume */
+/* todo: compute (load) launch  */
 function tap_proof_op_valid_in_privileged (o : tap_proof_op_t) : bool
 {
     // o == tap_proof_op_compute   || o == tap_proof_op_destroy   ||
     // o == tap_proof_op_enter     || o == tap_proof_op_exit      ||
     // o == tap_proof_op_launch    || o == tap_proof_op_resume    ||
     // o == tap_proof_op_pause     
-    false
+    // false
     // o == tap_proof_op_compute   
     // o == tap_proof_op_destroy   
     // o == tap_proof_op_enter     
-    // o == tap_proof_op_exit      
+    // o == tap_proof_op_exit       
     // o == tap_proof_op_launch    
     // o == tap_proof_op_resume    
     // o == tap_proof_op_pause    
